Fix build errors with TxnDiskAPI. Add concurrency to StatDB layer/impl.

src/Examples/StatDb/Impl.v
@@ -3,36 +3,53 @@ From Coq Require Import List.
 From RecoveryRefinement Require Export Lib.
 
 Module Var.
-  Inductive id := Sum | Count.
+  Inductive id := Sum | Count | Lock.
   Inductive Op : Type -> Type :=
   | Read (i:id) : Op nat
-  | Write (i:id) (v:nat) : Op unit .
-  Definition State := (nat * nat)%type.
+  | Write (i:id) (v:nat) : Op unit
+  | CAS (i:id) (vold: nat) (vnew:nat) : Op nat .
+  Definition State := (nat * nat * nat)%type.
 
   Definition get (i:id) : State -> nat :=
     match i with
-    | Sum => fun '(x, _) => x
-    | Count => fun '(_, y) => y
+    | Sum => fun '(x, _, _) => x
+    | Count => fun '(_, y, _) => y
+    | Lock => fun '(_, _, z) => z
     end.
 
   Definition set (i:id) (v:nat) : State -> State :=
     match i with
-    | Sum => fun '(_, y) => (v, y)
-    | Count => fun '(x, _) => (x, v)
+    | Sum => fun '(_, y, z) => (v, y, z)
+    | Count => fun '(x, _, z) => (x, v, z)
+    | Lock => fun '(x, y, _) => (x, y, v)
     end.
+
+  Import RelationNotations.
+  Definition cas (i: id) (vold: nat) (vnew: nat): RelationAlgebra.relation State State nat :=
+    v <- reads (get i);
+    if nat_eq_dec v vold then
+        puts (set i vnew);;
+        pure v
+    else
+        pure v.
 
   Definition dynamics : Dynamics Op State :=
     {| step T (op: Op T) :=
          match op with
          | Read i => reads (get i)
          | Write i v => puts (set i v)
+         | CAS i vold vnew => cas i vold vnew
          end;
        crash_step :=
-         puts (fun _ => (0, 0)); |}.
+         puts (fun _ => (0, 0, 0)); |}.
 
   Lemma crash_total_ok (s: State):
-    exists s', dynamics.(crash_step) s s' tt.
+    exists s', dynamics.(crash_step) s (Val s' tt).
   Proof. eexists; econstructor. Qed.
+
+  Lemma crash_non_err_ok (s: State) ret:
+    dynamics.(crash_step) s ret -> ret ≠ Err.
+  Proof. inversion 1; congruence. Qed.
 
   Definition l : Layer Op :=
     {| Layer.State := State;
@@ -40,7 +57,8 @@ Module Var.
        trace_proj := fun _ => nil;
        crash_preserves_trace := fun _ _ _ => eq_refl;
        crash_total := crash_total_ok;
-       initP := fun s => s = (0, 0)|}.
+       crash_non_err := crash_non_err_ok;
+       initP := fun s => s = (0, 0, 0)|}.
 End Var.
 
 Module DB.
@@ -59,8 +77,12 @@ Module DB.
          puts (fun _ => nil); |}.
 
   Lemma crash_total_ok (s: State):
-    exists s', dynamics.(crash_step) s s' tt.
+    exists s', dynamics.(crash_step) s (Val s' tt).
   Proof. eexists; econstructor. Qed.
+
+  Lemma crash_non_err_ok (s: State) ret:
+    dynamics.(crash_step) s ret -> ret ≠ Err.
+  Proof. inversion 1; congruence. Qed.
 
   Definition l : Layer Op :=
     {| Layer.State := State;
@@ -68,21 +90,34 @@ Module DB.
        trace_proj := fun _ => nil;
        crash_preserves_trace := fun _ _ _ => eq_refl;
        crash_total := crash_total_ok;
+       crash_non_err := crash_non_err_ok;
        initP := fun s => s = nil |}.
 End DB.
 
 Definition read i := Call (Var.Read i).
 Definition write i v := Call (Var.Write i v).
 
+Definition lock : proc Var.Op unit :=
+  Loop (fun (_ : unit) =>
+          x <- Call (Var.CAS Var.Lock 0 1);
+          Ret (if nat_eq_dec x 0 then
+                  DoneWithOutcome tt
+                else
+                  ContinueOutcome tt)
+       )%proc tt.
+Definition unlock : proc Var.Op unit := Call (Var.Write Var.Lock 0).
+
 Definition impl : LayerImpl Var.Op DB.Op :=
   {| compile_op T (op: DB.Op T) :=
        match op with
        | DB.Add n =>
-         (sum <- read Var.Sum; _ <- write Var.Sum (n + sum)%nat;
-       count <- read Var.Count; _ <- write Var.Count (1 + count)%nat;
-       Ret tt)%proc
+         (_ <- lock;
+          sum <- read Var.Sum; _ <- write Var.Sum (n + sum)%nat;
+          count <- read Var.Count; _ <- write Var.Count (1 + count)%nat;
+          unlock)%proc
        | DB.Avg =>
-         (sum <- read Var.Sum; count <- read Var.Count; Ret (sum/count)%nat)%proc
+         (_ <- lock;
+          sum <- read Var.Sum; count <- read Var.Count; _ <- unlock; Ret (sum/count)%nat)%proc
        end;
      recover := Seq_Cons (Ret tt) (Seq_Nil);
      (* init := Ret Initialized; *) |}.
