src/Examples/Logging/TxnDiskAPI.v
@@ -15,7 +15,7 @@ Module TxnD.
 
   Inductive op_step : OpSemantics Op State :=
   | step_commit : forall d_old d,
-      op_step (op_commit) (d_old, d) (d, d) tt
+      op_step (op_commit) (d_old, d) (Val (d, d) tt)
   | step_read : forall a r d_old d,
       (* note that we read from the old disk - this allows the log to serve
       reads directly from the data region rather than from the log (which in
@@ -24,27 +24,35 @@ Module TxnD.
       | Some b0 => r = b0
       | None => exists b, r = b
       end ->
-      op_step (op_read a) (d_old, d) (d_old, d) r
+      op_step (op_read a) (d_old, d) (Val (d_old, d) r)
   | step_write_success : forall a b d_old d d',
       d' = (assign d a b) ->
-      op_step (op_write a b) (d_old, d) (d_old, d') WriteOK
+      op_step (op_write a b) (d_old, d) (Val (d_old, d') WriteOK)
   | step_write_fail : forall a b d_old d,
-      op_step (op_write a b) (d_old, d) (d_old, d) WriteErr
+      op_step (op_write a b) (d_old, d) (Val (d_old, d) WriteErr)
   | step_size : forall d_old d,
       (* it's an invariant of the log that the disks have the same size *)
-      op_step (op_size) (d_old, d) (d_old, d) (length d).
+      op_step (op_size) (d_old, d) (Val (d_old, d) (length d)).
 
-  Definition txn_crash : State -> State -> unit -> Prop :=
-    fun '(d_old, d) '(d_old', d') r =>
-      d_old' = d_old /\
-      d' = d_old.
+  Definition txn_crash : RelationAlgebra.relation State State unit :=
+    fun '(d_old, d) ret =>
+      match ret with
+        | Val (d_old', d') r =>
+          d_old' = d_old /\
+          d' = d_old
+        | _ => False
+      end.
 
   Definition dyn : Dynamics Op State :=
     {| step := op_step; crash_step := txn_crash |}.
 
   Lemma crash_total_ok (s: State):
-    exists s', dyn.(crash_step) s s' tt.
+    exists s', dyn.(crash_step) s (Val s' tt).
   Proof. destruct s as (d1, d1'). exists (d1, d1). econstructor; eauto. Qed.
+
+  Lemma crash_non_err_ok (s: State) ret:
+    dyn.(crash_step) s ret -> ret ≠ Err.
+  Proof. destruct s, ret; auto. Qed.
 
   Definition l : Layer Op :=
     {| Layer.State := State;
@@ -52,6 +60,7 @@ Module TxnD.
        trace_proj := fun _ => nil;
        crash_preserves_trace := fun _ _ _ => eq_refl;
        crash_total := crash_total_ok;
+       crash_non_err := crash_non_err_ok;
        initP := fun '(d_old, d) => d_old = d |}.
 
 End TxnD.
